Refactored print failure in string parsers

src/Parsers/library.dfy
@@ -1,8 +1,12 @@
 module {:options "/functionSyntax:4"} Printer {
 
-  type stringNat = s: string |
+  predicate IsStringNat(s: string) {
     |s| > 0 && (|s| > 1 ==> s[0] != '0') &&
     forall i | 0 <= i < |s| :: s[i] in "0123456789"
+  }
+
+  type stringNat = s: string |
+    IsStringNat(s)
     witness "1"
 
   function natToString(n: nat): stringNat {
